wip

Untangle.v
@@ -10,6 +10,9 @@ Require Export SystemFR.TOpenTClose.
 Require Export SystemFR.CloseLemmas.
 Require Export SystemFR.SubstitutionErase.
 Require Export SystemFR.TermListReducible.
+Require Export SystemFR.ReducibilityOpenEquivalent.
+Require Export SystemFR.FVLemmasClose.
+Require Export SystemFR.WFLemmasClose.
 
 Opaque reducible_values.
 
@@ -58,8 +61,6 @@ Proof.
   repeat step || rewrite substitute_map || rewrite substitute_key.
 Qed.
 
-Opaque T_key.
-Opaque T_map.
 Opaque T_trail.
 
 Definition app2 f a b := app (app f a) b.
@@ -173,6 +174,20 @@ Hypothesis update_spec3:
 (* Terms that take a map and a key `k`, and only lookup the map on keys greater or
    equal than `k` satisfy the following property, described by the type `T_tau` *)
 Parameter T_tau: tree.
+
+Hypothesis tau_fv: forall tag, pfv T_tau tag = nil.
+Hypothesis wf_tau: wf T_tau 0.
+Hypothesis is_erased_type_tau: is_erased_type T_tau.
+
+Hint Resolve wf_tau: wf.
+Hint Resolve is_erased_type_tau: erased.
+
+Lemma substitute_tau:
+  forall l tag, psubstitute T_tau l tag = T_tau.
+Proof.
+  intros; apply substitute_nothing5; eauto using tau_fv.
+Qed.
+
 Lemma tau_property:
   forall f map key trail,
     [ f : T_tau ] ->
@@ -346,6 +361,14 @@ Proof.
   induction l1; destruct l2; repeat step || apply f_equal.
 Qed.
 
+Lemma range_combine:
+  forall A B (l1: list A) (l2: list B),
+    List.length l1 = List.length l2 ->
+    range (List.combine l1 l2) = l2.
+Proof.
+  induction l1; destruct l2; repeat step || apply f_equal.
+Qed.
+
 Lemma subst_subst2:
   forall t l ts xs tag,
     length ts = length xs ->
@@ -476,7 +499,215 @@ Proof.
   rewrite open_closes; steps; eauto with wf fv.
 Qed.
 
-Lemma reducible_exists_vars2:
+Definition functional { A B } (m: map A B) :=
+  forall a b1 b2,
+    (a, b1) ∈ m ->
+    (a, b2) ∈ m ->
+    b1 = b2.
+
+Lemma functional_head:
+  forall A B a b1 b2 (m: map A B),
+    functional ((a, b1) :: m) ->
+    (a, b2) ∈ m ->
+    b1 = b2.
+Proof.
+  unfold functional; steps; eauto.
+Qed.
+
+Lemma functional_trail:
+  forall A B a b (m: map A B),
+    functional ((a, b) :: m) ->
+    functional m.
+Proof.
+  unfold functional; steps; eauto.
+Qed.
+
+Ltac destruct_refinement :=
+  match goal with
+  | H: { _: _ | _ } |- _ => destruct H
+  | H: { _: _ & _ } |- _ => destruct H
+  end.
+
+Definition get_or_else { A } (opt: option A) (a: A) :=
+  match opt with
+  | None => a
+  | Some x => x
+  end.
+
+Lemma lookup_some_in:
+  forall A (l: map nat A) x a,
+    lookup Nat.eq_dec l x = Some a ->
+    (x, a) ∈ l.
+Proof.
+  induction l; steps.
+Qed.
+
+Lemma in_map_in_support:
+  forall A B (l: map A B) p,
+    p ∈ l ->
+    (fst p) ∈ support l.
+Proof.
+  induction l; steps.
+Qed.
+
+Lemma functional_get_or_else:
+  forall T a b (m: map nat T),
+    functional m ->
+    functional (m ++ (a, get_or_else (lookup Nat.eq_dec m a) b) :: nil).
+Proof.
+  unfold functional, get_or_else;
+    repeat step || list_utils || t_lookup; eauto;
+    try solve [ apply_anywhere lookup_some_in; steps; eauto ];
+    try solve [ apply_anywhere in_map_in_support; steps; eauto ];
+    eauto using in_combine_l with exfalso.
+Qed.
+
+Lemma decide_empty:
+  forall T (l: list T), l = nil \/ ~ l = nil.
+Proof.
+  destruct l; steps; right; steps.
+Qed.
+
+Lemma lookup_support:
+  forall A (l: map nat A) x,
+   x ∈ support l ->
+   exists a, lookup Nat.eq_dec l x = Some a.
+Proof.
+  induction l; repeat step; eauto.
+Qed.
+
+Lemma lookup_support2:
+  forall A (l1 l2: map nat A) x,
+   (forall s t, lookup Nat.eq_dec l1 s = Some t <-> lookup Nat.eq_dec l2 s = Some t) ->
+   x ∈ support l1 ->
+   x ∈ support l2.
+Proof.
+  intros.
+  apply_anywhere lookup_support; repeat step.
+  pose proof (H x a); repeat step || t_lookup.
+Qed.
+
+Lemma equivalent_subst_snoc:
+  forall l1 l2 a b,
+    equivalent_subst l1 l2 ->
+    equivalent_subst
+      (l1 ++ (a, b) :: nil)
+      (l2 ++ (a, get_or_else (lookup Nat.eq_dec l2 a) b) :: nil).
+Proof.
+  unfold equivalent_subst, get_or_else;
+    repeat step || list_utils || t_lookup || t_lookupor ||
+           (rewrite obvious_lookup in * by auto);
+    try solve [ apply lookupWeaken; steps; apply_any; steps ];
+    try solve [ unshelve epose proof (H s _); eauto; steps ].
+
+  - rewrite obvious_lookup in *; repeat step || t_lookup.
+    + apply eq_sym in H8; unshelve epose proof (H s b); repeat step || t_lookup.
+    + clear_marked. rewrite H8 in H0.
+      unshelve epose proof (H s t); repeat step || t_lookup.
+  - apply obvious_lookup; repeat step; eauto using lookup_support2.
+Qed.
+
+Lemma support_nil:
+  forall A B (l: map A B), support l = nil <-> l = nil.
+Proof.
+  destruct l; steps.
+Qed.
+
+Lemma forall_inst:
+  forall A (P: A -> Prop) l x,
+    x ∈ l ->
+    Forall P l ->
+    P x.
+Proof.
+  repeat step || rewrite Forall_forall in *.
+Qed.
+
+Ltac forall_inst :=
+  match goal with
+  | H1: ?x ∈ ?l, H2: Forall ?P ?l |- _ =>
+    poseNew (Mark (x, H2) "forall_inst");
+    pose proof (forall_inst _ _ _ _ H1 H2)
+  end.
+
+Lemma range_append:
+  forall A B (l1 l2: map A B),
+    range (l1 ++ l2) = range l1 ++ range l2.
+Proof.
+  induction l1; repeat step.
+Qed.
+
+Lemma recombine:
+  forall A B (m: map A B),
+    combine (support m) (range m) = m.
+Proof.
+  induction m; steps.
+Qed.
+
+Lemma length_support:
+  forall A B (l: map A B), length (support l) = length l.
+Proof.
+  induction l; steps.
+Qed.
+
+Lemma length_range:
+  forall A B (l: map A B), length (range l) = length l.
+Proof.
+  induction l; steps.
+Qed.
+
+Ltac list_utils2 :=
+  rewrite map_length in * || rewrite support_nil in * || rewrite in_map_iff in * ||
+  rewrite range_append in * || rewrite range_combine in * ||
+  rewrite List.map_map in * || rewrite support_combine in * ||
+  rewrite length_support in * || rewrite length_range in * ||
+  rewrite length_zero_iff_nil in * ||
+  rewrite recombine in * ||
+  forall_inst.
+
+Lemma functionalize_helper:
+  forall n (l: map nat tree),
+   length l < n ->
+   exists l',
+     functional l' /\
+      (forall y, y ∈ range l' -> y ∈ range l) /\
+     support l = support l' /\
+     equivalent_subst l l'.
+Proof.
+  induction n; steps; try lia.
+  pose proof (decide_empty _ l); steps.
+  - unfold functional, equivalent_subst; exists nil; steps.
+  - unshelve epose proof (@exists_last _ l _);
+      repeat step || destruct_refinement.
+    unshelve epose proof (IHn x _); repeat step || rewrite app_length in *; try lia.
+    exists (l' ++ (n0, get_or_else (lookup Nat.eq_dec l' n0) t) :: nil);
+      repeat step || apply equivalent_subst_snoc || list_utils || list_utils2;
+      eauto 2 using functional_get_or_else.
+    unfold get_or_else; steps; eauto using lookupRange.
+Qed.
+
+Lemma functionalize:
+  forall (l: map nat tree),
+    exists l',
+      functional l' /\
+      (forall y, y ∈ range l' -> y ∈ range l) /\
+      support l = support l' /\
+      equivalent_subst l l'.
+Proof.
+  eauto using functionalize_helper.
+Qed.
+
+Lemma functionalize_subst:
+  forall t l tag,
+  exists l',
+    functional l' /\
+    psubstitute t l tag = psubstitute t l' tag.
+Proof.
+  intros.
+  pose proof (functionalize l); steps;
+    eauto using subst_permutation.
+Qed.
+
+Lemma reducible_exists_vars2_helper:
   forall xs ρ v T1 T2,
     wf T1 0 ->
     wf T2 0 ->
@@ -487,9 +718,11 @@ Lemma reducible_exists_vars2:
     (exists vs,
       List.Forall (fun v => [ ρ | v : T1 ]v) vs /\
       length vs = length xs /\
-      [ ρ | v : psubstitute T2 (List.combine xs vs) term_var ]v).
+      [ ρ | v : psubstitute T2 (combine xs vs) term_var ]v).
 Proof.
-  induction xs; repeat step || t_substitutions || simp_red_top_level_hyp; eauto.
+  unfold functional; induction xs; repeat step || t_substitutions || simp_red_top_level_hyp;
+    eauto 2 with step_tactic.
+
   rewrite open_existss in *; eauto with wf.
   rewrite <- rev_length in * at 2.
   rewrite open_closes in *; eauto with wf fv.
@@ -499,27 +732,213 @@ Proof.
     eauto 2 with wf step_tactic;
     eauto 2 with erased step_tactic.
 
-  exists (a0 :: vs); steps.
+  exists (a0 :: vs); steps; eauto.
   rewrite substitute_cons2; repeat step || (erewrite reducible_val_fv in * by eauto).
+Qed.
+
+Lemma reducible_exists_vars2:
+  forall xs ρ v T1 T2,
+    wf T1 0 ->
+    wf T2 0 ->
+    is_erased_type T1 ->
+    is_erased_type T2 ->
+    valid_interpretation ρ ->
+    [ ρ | v : T_exists_vars xs T1 T2 ]v ->
+    (exists vs,
+      List.Forall (fun v => [ ρ | v : T1 ]v) vs /\
+      functional (combine xs vs) /\
+      length vs = length xs /\
+      [ ρ | v : psubstitute T2 (combine xs vs) term_var ]v).
+Proof.
+  intros.
+  apply_anywhere reducible_exists_vars2_helper; steps.
+  pose proof (functionalize (combine xs vs)); repeat step || list_utils2.
+  exists (range l'); repeat step || list_utils || list_utils2 || rewrite Forall_forall in *.
+  erewrite subst_permutation in * |-; eauto.
 Qed.
 
 Definition apps fs ts := List.map (fun p => app (fst p) (snd p)) (combine fs ts).
 
-(* Using the tau property, we can untangle *)
-Inductive untangle: context -> tree -> tree -> Prop :=
-| UntangleFreshen:
-    forall Γ T T' template xs ys fs keys m,
-      List.NoDup (xs ++ ys) ->
-      T  = substitute template
-        (List.combine xs (apps fs (List.map (fun key => pp key (fvar m term_var)) keys))) ->
-      T' = substitute template
-        (List.combine xs (apps fs (List.map (fun y => fvar y term_var) ys))) ->
-      untangle Γ
-               (T_exists T_trail (close 0 T m))
-               (T_exists_vars ys T_trail T')
+Lemma combine_equivalent_wfs1:
+  forall ts1 ts2 xs,
+    length xs = length ts1 ->
+    length xs = length ts2 ->
+    (forall t1 t2, (t1, t2) ∈ combine ts1 ts2 -> [ t1 ≡ t2 ]) ->
+    wfs (combine xs ts1) 0.
+Proof.
+  induction ts1; destruct ts2; destruct xs;
+    repeat step || list_utils || list_utils2; eauto.
+  unshelve epose proof (H1 a t _); steps; t_closer.
+Qed.
 
-| UntangleRefl: forall Γ T, untangle Γ T T
-.
+Lemma combine_equivalent_wfs2:
+  forall ts1 ts2 xs,
+    length xs = length ts1 ->
+    length xs = length ts2 ->
+    (forall t1 t2, (t1, t2) ∈ combine ts1 ts2 -> [ t1 ≡ t2 ]) ->
+    wfs (combine xs ts2) 0.
+Proof.
+  induction ts1; destruct ts2; destruct xs;
+    repeat step || list_utils || list_utils2; eauto.
+  unshelve epose proof (H1 a t _); steps; t_closer.
+Qed.
+
+Lemma combine_wfs3:
+  forall xs ts,
+    (forall x t, (x, t) ∈ combine xs ts -> wf t 0) ->
+    wfs (combine xs ts) 0.
+Proof.
+  induction xs; destruct ts;
+    repeat step || list_utils || list_utils2; eauto.
+Qed.
+
+Lemma combine_wfs4:
+  forall xs ts,
+    (forall t, t ∈ ts -> wf t 0) ->
+    wfs (combine xs ts) 0.
+Proof.
+  induction xs; destruct ts;
+    repeat step || list_utils || list_utils2; eauto.
+Qed.
+
+Lemma combine_wfs5:
+  forall xs ts,
+    Forall (fun v => wf v 0) ts ->
+    wfs (combine xs ts) 0.
+Proof.
+  intros; apply combine_wfs4; apply Forall_forall; auto.
+Qed.
+
+Lemma combine_equivalent_is_erased_term:
+  forall xs ts,
+    Forall is_erased_term ts ->
+    erased_terms (combine xs ts).
+Proof.
+  induction xs; destruct ts;
+    repeat step || list_utils || list_utils2; eauto.
+Qed.
+
+Lemma combine_closed_mapping:
+  forall xs ts tag,
+    Forall (fun t => pfv t tag = nil) ts ->
+    pclosed_mapping (combine xs ts) tag.
+Proof.
+  induction xs; destruct ts;
+    repeat step || list_utils || list_utils2; eauto.
+Qed.
+
+Lemma pfv_in_subst2:
+  forall T (l : list (nat * tree)) tag x,
+    pclosed_mapping l tag ->
+    x ∈ pfv (psubstitute T l tag) tag ->
+    ~x ∈ support l.
+Proof.
+  intros.
+  epose proof (fv_subst2 _ _ _ x H0);
+    repeat step || list_utils;
+    eauto using closed_mapping_fv.
+Qed.
+
+Lemma reducibility_equivalent_substititions_helper:
+  forall xs T ρ v ts1 ts2,
+    [ ρ | v : psubstitute T (combine xs ts1) term_var ]v ->
+    valid_interpretation ρ ->
+    length ts1 = length xs ->
+    length ts2 = length xs ->
+    is_erased_type T ->
+    wf T 0 ->
+    (forall t1 t2, (t1, t2) ∈ combine ts1 ts2 -> [ t1 ≡ t2 ]) ->
+    Forall (fun v => wf v 0) ts1 ->
+    Forall (fun v => wf v 0) ts2 ->
+    Forall (fun v => pfv v term_var = nil) ts1 ->
+    Forall (fun v => pfv v term_var = nil) ts2 ->
+    Forall is_erased_term ts1 ->
+    Forall is_erased_term ts2 ->
+    (forall x, x ∈ fv T -> x ∈ xs) ->
+    [ ρ | v : psubstitute T (combine xs ts2) term_var ]v.
+Proof.
+  induction xs; repeat step || t_substitutions.
+  rewrite <- (open_close2 T a 0) by auto.
+  rewrite substitute_open3; steps;
+    try solve [ apply combine_equivalent_wfs4; repeat step || rewrite Forall_forall in *; eauto ];
+    try solve [ apply_anywhere fv_close; steps ].
+
+  eapply reducibility_open_equivalent; eauto;
+    repeat step || apply subst_erased_type || apply wf_subst || apply wf_close;
+    eauto with erased wf fv;
+    eauto using combine_equivalent_is_erased_term.
+
+  - rewrite substitute_open2;
+      repeat step || list_utils || list_utils2 ||
+             rewrite open_close by auto;
+      eauto using combine_wfs5.
+    apply IHxs with l0;
+      repeat step || apply subst_erased_type || apply wf_subst || t_pfv_in_subst;
+      eauto.
+    + rewrite <- substitute_cons; steps.
+    + clear_marked; apply pfv_in_subst2 in H6; steps.
+      instantiate_any; steps.
+  - apply wfs_monotone2.
+    apply combine_wfs4; repeat step || rewrite Forall_forall in *; eauto with wf.
+  - apply fv_nils2; repeat step || list_utils2 || unfold subset || apply_anywhere fv_close;
+      eauto using combine_closed_mapping.
+    apply_anywhere H12; steps.
+  - apply combine_wfs5; auto.
+Qed.
+
+Lemma find_snd:
+  forall A B a (l1: list A) (l2: list B),
+    a ∈ l1 ->
+    length l1 = length l2 ->
+    exists b, (a, b) ∈ combine l1 l2.
+Proof.
+  induction l1; repeat step || instantiate_any; eauto.
+  pose proof (IHl1 _ H1 H); steps; eauto.
+Qed.
+
+Ltac find_snd :=
+  match goal with
+  | H1: context[combine ?l1 ?l2],
+    H2: ?x ∈ ?l1 |- _ =>
+    poseNew (Mark (x, l1, l2) "first_snd");
+    unshelve epose proof (find_snd _ _ _ l1 l2 H2 _)
+  end.
+
+Lemma find_fst:
+  forall A B b (l1: list A) (l2: list B),
+    b ∈ l2 ->
+    length l1 = length l2 ->
+    exists a, (a, b) ∈ combine l1 l2.
+Proof.
+  induction l1; repeat step || instantiate_any; eauto.
+  apply_anywhere eq_sym; list_utils2; steps.
+Qed.
+
+Ltac find_fst :=
+  match goal with
+  | H1: context[combine ?l1 ?l2],
+    H2: ?x ∈ ?l2 |- _ =>
+    poseNew (Mark (x, l1, l2) "first_fst");
+    unshelve epose proof (find_fst _ _ _ l1 l2 H2 _)
+  end.
+
+Lemma reducibility_equivalent_substititions:
+  forall xs T ρ v ts1 ts2,
+    [ ρ | v : psubstitute T (combine xs ts1) term_var ]v ->
+    valid_interpretation ρ ->
+    length ts1 = length xs ->
+    length ts2 = length xs ->
+    is_erased_type T ->
+    wf T 0 ->
+    (forall t1 t2, (t1, t2) ∈ combine ts1 ts2 -> [ t1 ≡ t2 ]) ->
+    (forall x, x ∈ fv T -> x ∈ xs) ->
+    [ ρ | v : psubstitute T (combine xs ts2) term_var ]v.
+Proof.
+  intros; eapply reducibility_equivalent_substititions_helper; try eassumption;
+    repeat step || rewrite Forall_forall || find_fst || find_snd;
+    eauto using combine_equivalent_wfs1;
+    try solve [ instantiate_any; t_closer ].
+Qed.
 
 Lemma erased_terms_combine:
   forall xs f ys,
@@ -659,33 +1078,6 @@ Proof.
   induction keys; repeat step || constructor; eauto using append_key_trail.
 Qed.
 
-Lemma support_nil:
-  forall A B (l: map A B), support l = nil <-> l = nil.
-Proof.
-  destruct l; steps.
-Qed.
-
-Lemma forall_inst:
-  forall A (P: A -> Prop) l x,
-    x ∈ l ->
-    Forall P l ->
-    P x.
-Proof.
-  repeat step || rewrite Forall_forall in *.
-Qed.
-
-Ltac forall_inst :=
-  match goal with
-  | H1: ?x ∈ ?l, H2: Forall ?P ?l |- _ =>
-    poseNew (Mark (x, H2) "forall_inst");
-    pose proof (forall_inst _ _ _ _ H1 H2)
-  end.
-
-Ltac list_utils2 :=
-  rewrite map_length in * || rewrite support_nil in * || rewrite in_map_iff in * ||
-  rewrite List.map_map in * || rewrite support_combine in * ||
-  forall_inst.
-
 Lemma list_map_subst4:
   forall keys a l,
     Forall (fun key : tree => [key : T_key ]v) keys ->
@@ -741,18 +1133,20 @@ Qed.
 Lemma lookup_combine:
   forall A B (l1: list nat) (l2: list A) x a (f: A -> B),
     length l1 = length l2 ->
-    NoDup l1 ->
+    functional (combine l1 l2) ->
     (x, a) ∈ combine l1 l2 ->
     lookup Nat.eq_dec (combine l1 (List.map f l2)) x = Some (f a).
 Proof.
   induction l1; destruct l2; repeat step || step_inversion NoDup;
-    eauto using in_combine_l with exfalso.
+    eauto using in_combine_l with exfalso;
+    try solve [ eapply_anywhere functional_head; eauto; steps ];
+    eauto using functional_trail.
 Qed.
 
 Lemma list_map_subst7:
   forall ys keys a,
     length ys = length keys ->
-    NoDup ys ->
+    functional (combine ys keys) ->
     List.map
       (fun y =>
          match
@@ -772,18 +1166,20 @@ Qed.
 Lemma lookup_combine2:
   forall A B (l1: list nat) (l2: list A) x a (f: A -> B),
     length l1 = length l2 ->
-    NoDup l1 ->
+    functional (combine l1 l2) ->
     (x, a) ∈ combine l1 l2 ->
     lookup Nat.eq_dec (combine l1 l2) x = Some a.
 Proof.
   induction l1; destruct l2; repeat step || step_inversion NoDup;
-    eauto using in_combine_l with exfalso.
+    eauto using in_combine_l with exfalso;
+    try solve [ eapply_anywhere functional_head; eauto; steps ];
+    eauto using functional_trail.
 Qed.
 
 Lemma list_map_subst8:
   forall ys vs l,
     length vs = length ys ->
-    NoDup ys ->
+    functional (combine ys vs) ->
     (forall y, y ∈ ys -> y ∈ support l -> False) ->
     List.map
       (fun x =>
@@ -803,6 +1199,243 @@ Qed.
 
 (* empty_trail: T_trail *)
 Parameter empty_trail: tree.
+Hypothesis empty_trail_type: [ empty_trail : T_trail ]v.
+
+Definition global_trail keys vs :=
+  fold_left (fun acc p => update acc (fst p) (snd p)) (combine keys vs) empty_trail.
+
+Lemma is_erased_term_global_trail':
+  forall keys vs acc0,
+    is_erased_term acc0 ->
+    Forall is_erased_term keys ->
+    Forall is_erased_term vs ->
+    is_erased_term (fold_left (fun acc p => update acc (fst p) (snd p)) (combine keys vs) acc0).
+Proof.
+  induction keys; repeat step || apply_any; eauto with erased.
+Qed.
+
+Lemma wfs_global_trail':
+  forall keys vs acc0,
+    wf acc0 0 ->
+    Forall (fun v => wf v 0) keys ->
+    Forall (fun v => wf v 0) vs ->
+    wf (fold_left (fun acc p => update acc (fst p) (snd p)) (combine keys vs) acc0) 0.
+Proof.
+  induction keys; repeat step || apply_any; eauto with wf.
+Qed.
+
+Lemma fvs_global_trail':
+  forall keys vs acc0 tag,
+    pfv acc0 tag = nil ->
+    Forall (fun v => pfv v tag = nil) keys ->
+    Forall (fun v => pfv v tag = nil) vs ->
+    pfv (fold_left (fun acc p => update acc (fst p) (snd p)) (combine keys vs) acc0) tag = nil.
+Proof.
+  induction keys; repeat step || apply_any || rewrite pfv_update || list_utils.
+Qed.
+
+Lemma global_trail_is_trail':
+  forall keys vs acc0,
+    [ acc0 : T_trail ]v  ->
+    Forall (fun key => [ key : T_key ]v) keys ->
+    Forall (fun trail => [ trail : T_trail ]v) vs ->
+    [ fold_left (fun acc p => update acc (fst p) (snd p)) (combine keys vs) acc0 : T_trail ]v.
+Proof.
+  induction keys; repeat step || apply_any; eauto using update_type.
+Qed.
+
+Lemma typed_erased_terms:
+  forall ρ T l,
+    valid_interpretation ρ ->
+    Forall (fun v => [ ρ | v : T ]v) l ->
+    Forall is_erased_term l.
+Proof.
+  induction l; repeat step || constructor;
+    try solve [ eapply reducible_values_erased; eauto using empty_trail_type; steps ].
+Qed.
+
+Lemma typed_erased_terms':
+  forall T l,
+    Forall (fun v => [ v : T ]v) l ->
+    Forall is_erased_term l.
+Proof.
+  intros; eapply typed_erased_terms; eauto; steps.
+Qed.
+
+Lemma typed_wfs:
+  forall ρ T l,
+    valid_interpretation ρ ->
+    Forall (fun v => [ ρ | v : T ]v) l ->
+    Forall (fun v => wf v 0) l.
+Proof.
+  induction l; repeat step || constructor;
+    try solve [ eapply reducible_val_wf; eauto using empty_trail_type; steps ].
+Qed.
+
+Lemma typed_wfs':
+  forall T l,
+    Forall (fun v => [ v : T ]v) l ->
+    Forall (fun v => wf v 0) l.
+Proof.
+  intros; eapply typed_wfs; eauto; steps.
+Qed.
+
+Lemma typed_fv:
+  forall ρ T l tag,
+    valid_interpretation ρ ->
+    Forall (fun v => [ ρ | v : T ]v) l ->
+    Forall (fun v => pfv v tag = nil) l.
+Proof.
+  induction l; repeat step || constructor;
+    try solve [ eapply reducible_val_fv; eauto using empty_trail_type; steps ].
+Qed.
+
+Lemma typed_fv':
+  forall T l tag,
+    Forall (fun v => [ v : T ]v) l ->
+    Forall (fun v => pfv v tag = nil) l.
+Proof.
+  intros; eapply typed_fv; eauto; steps.
+Qed.
+
+Lemma is_erased_term_global_trail:
+  forall keys vs,
+    Forall is_erased_term keys ->
+    Forall is_erased_term vs ->
+    is_erased_term (global_trail keys vs).
+Proof.
+  intros; apply is_erased_term_global_trail'; steps;
+    try solve [ eapply reducible_values_erased; eauto using empty_trail_type; steps ].
+Qed.
+
+Lemma wfs_global_trail:
+  forall keys vs,
+    Forall (fun v => wf v 0) keys ->
+    Forall (fun v => wf v 0) vs ->
+    wf (global_trail keys vs) 0.
+Proof.
+  intros; apply wfs_global_trail'; steps;
+    try solve [ eapply reducible_val_wf; eauto using empty_trail_type; steps ].
+Qed.
+
+Lemma fvs_global_trail:
+  forall keys vs tag,
+    Forall (fun v => pfv v tag = nil) keys ->
+    Forall (fun v => pfv v tag = nil) vs ->
+    pfv (global_trail keys vs) tag = nil.
+Proof.
+  intros; apply fvs_global_trail'; steps;
+    try solve [ eapply reducible_val_fv; eauto using empty_trail_type; steps ].
+Qed.
+
+Lemma fvs_global_trail2:
+  forall keys vs tag x,
+    Forall (fun key => [ key : T_key ]v) keys ->
+    Forall (fun trail => [ trail : T_trail ]v) vs ->
+    x ∈ pfv (global_trail keys vs) tag ->
+    False.
+Proof.
+  intros; rewrite fvs_global_trail in *; steps; eauto using typed_fv'.
+Qed.
+
+Lemma global_trail_is_trail:
+  forall keys vs,
+    Forall (fun key => [ key : T_key ]v) keys ->
+    Forall (fun trail => [ trail : T_trail ]v) vs ->
+    [ global_trail keys vs : T_trail ]v.
+Proof.
+  intros; apply global_trail_is_trail'; steps; eauto using empty_trail_type.
+Qed.
+
+
+Definition good_trail (trail: tree) (key: tree) (trail': tree) : Prop :=
+  forall f,
+    [ f: T_tau ] ->
+    [ app f trail' ≡ app f (append_key key trail) ].
+
+Lemma good_trail_equivalent:
+  forall key trail trail' f,
+    good_trail trail key trail' ->
+    [ f : T_tau ] ->
+    [ app f trail' ≡ app f (append_key key trail) ].
+Proof.
+  unfold good_trail; steps.
+Qed.
+
+Lemma global_trail_good_trail':
+  forall keys vs key v acc,
+    length keys = length vs ->
+    (key, v) ∈ combine keys vs ->
+    good_trail (fold_left (fun acc p => update acc (fst p) (snd p)) (combine keys vs) acc) key v.
+Proof.
+  induction keys; destruct vs; repeat step.
+  
+Admitted.
+
+Lemma global_trail_good_trail:
+  forall keys vs key v,
+    length keys = length vs ->
+    (key, v) ∈ combine keys vs ->
+    good_trail (global_trail keys vs) key v.
+Proof.
+  intros; apply global_trail_good_trail'; steps.
+Qed.
+
+Opaque global_trail.
+
+(* Using the tau property, we can untangle *)
+Inductive untangle: context -> tree -> tree -> Prop :=
+| UntangleFreshen:
+    forall Γ T T' template xs ys fs keys m,
+      List.NoDup (xs ++ ys) ->
+      T  = substitute template
+        (List.combine xs (apps fs (List.map (fun key => pp key (fvar m term_var)) keys))) ->
+      T' = substitute template
+        (List.combine xs (apps fs (List.map (fun y => fvar y term_var) ys))) ->
+      untangle Γ
+               (T_exists T_trail (close 0 T m))
+               (T_exists_vars ys T_trail T')
+
+| UntangleRefl: forall Γ T, untangle Γ T T
+.
+
+Lemma in_combine_equivalent:
+  forall fs keys vs t1 l t2 trail,
+    length fs = length vs ->
+    length fs = length keys ->
+    (forall f, f ∈ fs -> [ psubstitute f l term_var : T_tau ]) ->
+    (forall key v, (key, v) ∈ combine keys vs -> good_trail trail key v) ->
+    (t1, t2) ∈
+      combine
+        (apps (List.map (fun f => psubstitute f l term_var) fs) vs)
+        (apps (List.map (fun f => psubstitute f l term_var) fs)
+          (List.map (fun x => append_key x trail) keys)) ->
+    [t1 ≡ t2].
+Proof.
+  induction fs; destruct keys; destruct vs;
+    repeat rewrite apps_cons in * || step;
+    try solve [ apply IHfs with keys vs l trail; steps ].
+
+  unshelve epose proof (H1 a _); steps.
+  unshelve epose proof (H2 t t0 _); steps;
+    eauto using good_trail_equivalent.
+Qed.
+
+Lemma in_combine_equivalent':
+  forall fs keys vs t1 l t2,
+    length fs = length vs ->
+    length fs = length keys ->
+    (forall f, f ∈ fs -> [ psubstitute f l term_var : T_tau ]) ->
+    (t1, t2) ∈
+      combine
+        (apps (List.map (fun f => psubstitute f l term_var) fs) vs)
+        (apps (List.map (fun f => psubstitute f l term_var) fs)
+          (List.map (fun x => append_key x (global_trail keys vs)) keys)) ->
+    [t1 ≡ t2].
+Proof.
+  intros; apply in_combine_equivalent with fs keys vs l (global_trail keys vs); steps;
+    eauto using global_trail_good_trail.
+Qed.
 
 Lemma untangle_freshen:
   forall Γ fs template xs ys keys m,
@@ -812,16 +1445,18 @@ Lemma untangle_freshen:
     Forall (fun key => [ key : T_key ]v) keys ->
     Forall (fun f => wf f 0) fs ->
     Forall is_erased_term fs ->
+    functional (combine ys keys) ->
     ~ m ∈ fv template ->
     length keys = length xs ->
     length fs = length xs ->
     length ys = length xs ->
-    NoDup ys ->
     (forall f, f ∈ fs -> m ∈ fv f -> False) ->
     (forall y, y ∈ ys -> y ∈ support Γ -> False) ->
     (forall y, y ∈ ys -> y ∈ fv template -> False) ->
     (forall x, x ∈ xs -> x ∈ support Γ -> False) ->
     (forall f, f ∈ fs -> subset (fv f) (support Γ)) ->
+    (forall f, f ∈ fs -> [ Γ ⊨ f : T_tau ]) ->
+    (forall x, x ∈ fv template -> x ∈ xs \/ x ∈ support Γ) ->
     [Γ
     ⊨ T_exists T_trail
         (close 0
@@ -927,21 +1562,45 @@ Proof.
       try solve [ eapply satisfies_erased_terms; eauto; steps ];
       try solve [ eapply reducible_values_closed; eauto; steps ].
 
+     exists (global_trail keys vs); repeat step;
+       eauto using typed_erased_terms', is_erased_term_global_trail;
+       eauto using typed_fv', fvs_global_trail;
+       eauto using typed_wfs', wfs_global_trail;
+       eauto using global_trail_is_trail.
 
-Definition global_trail keys vs :=
-  fold_left (fun acc p => update acc (fst p) (snd p)) (combine keys vs) empty_trail.
+    rewrite substitute_open2 in *; repeat step || list_utils; eauto with wf;
+      eauto using fvs_global_trail2.
+    rewrite open_close in *; steps; eauto using wfs_combine7 with wf.
+    rewrite (subst_subst template);
+      repeat step || t_substitutions ||
+             (rewrite substitute_nothing6 in * by auto) ||
+             (rewrite list_map_apps in * by repeat step || list_utils2) ||
+             rewrite List.map_map in *.
+    rewrite list_map_subst3 in *; steps; eauto.
 
-    exists (global_trail keys vs); steps.
+    rewrite (subst_subst2 template);
+      repeat step || list_utils2 || rewrite list_map_subst4 in * ||
+             (rewrite length_apps by (repeat step || list_utils2)) ||
+             (rewrite list_map_apps in * by repeat step || list_utils2);
+      eauto using var_in_support;
+      eauto with fv;
+      eauto using global_trail_is_trail.
 
-    global_trail keys vs.
-    apply reducible_exists.
-    define global_trail
-      (fold_left (fun acc p => update acc (fst p) (snd p)) (combine keys vs) empty_trail).
+    eapply reducibility_equivalent_substititions; try eassumption;
+      repeat step || list_utils || list_utils2 || apply subst_erased_type ||
+             t_pfv_in_subst ||
+             rewrite length_apps by (repeat step || list_utils2);
+      eauto with erased wf fv;
+      try solve [ eapply satisfies_erased_terms; eauto; steps ].
 
+    + apply in_combine_equivalent' with fs keys vs l; steps.
+      unfold open_reducible in *; repeat step.
+      unshelve epose proof (H15 f _ nil l _ _ _);
+        repeat step || rewrite substitute_tau in *.
 
-
-    admit.
-Admitted.
+    + instantiate_any; steps.
+      clear_marked; apply_anywhere pfv_in_subst2; steps; eauto with fv.
+Qed.
 
 Lemma untangle_open_equivalent_types:
   forall Γ T1 T2,
@@ -949,12 +1608,6 @@ Lemma untangle_open_equivalent_types:
     [ Γ ⊨ T1 = T2 ].
 Proof.
   induction 1; eauto using open_equivalent_types_refl; steps.
-
-
-  
-
-
-  
 Admitted.
 
 (*
